More work on Sec 3.5

analysis/Analysis/Section_3_1.lean
@@ -54,7 +54,7 @@ class SetTheory where
   regularity_axiom A (hA : ∃ x, mem x A) : ∃ x, mem x A ∧ ∀ S, x = set_to_object S → ¬ ∃ y, mem y A ∧ mem y S -- Axiom 3.9
   pow : Set → Set → Set -- Axiom 3.11
   function_to_object (X: Set) (Y: Set) : (Subtype (mem . X) → Subtype (mem . Y)) ↪ Object -- Axiom 3.11
-  power_set_axiom (X: Set) (Y: Set) (F:Object) : mem F (pow X Y) ↔ ∃ f: Subtype (mem . X) → Subtype (mem . Y), function_to_object X Y f = F -- Axiom 3.11
+  power_set_axiom (X: Set) (Y: Set) (F:Object) : mem F (pow X Y) ↔ ∃ f: Subtype (mem . Y) → Subtype (mem . X), function_to_object Y X f = F -- Axiom 3.11
   union : Set → Set -- Axiom 3.12
   union_axiom A x : mem x (union A) ↔ ∃ S, mem x S ∧ mem (set_to_object S) A -- Axiom 3.12
 
@@ -142,7 +142,11 @@ theorem SetTheory.Set.pair_eq (a b:Object) : ({a,b}:Set) = {a} ∪ {b} := by rfl
 /-- Axiom 3.3(b) (pair).  Note that one often has to cast {a,b} to Set -/
 @[simp]
 theorem SetTheory.Set.mem_pair (x a b:Object) : x ∈ ({a,b}:Set) ↔ (x = a ∨ x = b) := by
-  rw [pair_eq, mem_union, mem_singleton, mem_singleton]
+  simp [pair_eq, mem_union, mem_singleton]
+
+@[simp]
+theorem SetTheory.Set.mem_triple (x a b:Object) : x ∈ ({a,b,c}:Set) ↔ (x = a ∨ x = b ∨ x = c) := by
+  simp [Insert.insert, mem_union, mem_singleton]
 
 /-- Remark 3.1.8 -/
 theorem SetTheory.Set.singleton_uniq (a:Object) : ∃! (X:Set), ∀ x, x ∈ X ↔ x = a := by sorry
@@ -296,6 +300,19 @@ theorem SetTheory.Set.specification_axiom {A:Set} {P: A → Prop} {x:Object} (h:
 /-- Axiom 3.6 (axiom of specification) -/
 theorem SetTheory.Set.specification_axiom' {A:Set} (P: A → Prop) (x:A.toSubtype) : x.val ∈ A.specify P ↔ P x :=
   (SetTheory.specification_axiom A P).2 x
+
+/-- Axiom 3.6 (axiom of specification) -/
+theorem SetTheory.Set.specification_axiom'' {A:Set} (P: A → Prop) (x:Object) : x ∈ A.specify P ↔ ∃ h:x ∈ A, P ⟨ x, h ⟩ := by
+  constructor
+  . intro h
+    have h' := specification_axiom h
+    use h'
+    rw [←specification_axiom' P ⟨ x, h' ⟩ ]
+    simp [h]
+  intro h
+  obtain ⟨ h, hP ⟩ := h
+  rw [←specification_axiom' P ⟨ x,h ⟩ ] at hP
+  simp at hP; assumption
 
 theorem SetTheory.Set.specify_subset {A:Set} (P: A → Prop) : A.specify P ⊆ A := by sorry
 
